{
 "cells": [
  {
   "cell_type": "markdown",
   "id": "2b384ae4",
   "metadata": {
    "ExecuteTime": {
     "end_time": "2021-06-09T23:45:34.616014Z",
     "start_time": "2021-06-09T23:45:34.607098Z"
    }
   },
   "source": [
    "# Separation of Variables Cylindral Coordinates"
   ]
  },
  {
   "cell_type": "markdown",
   "id": "569f2e16",
   "metadata": {},
   "source": [
    "We will start with the general time-dependent diffusion equation\n",
    "\\begin{equation}\n",
    "\\nabla^2 u(\\rho, \\phi, t)  = \\frac {\\partial u}{\\partial t}\n",
    "\\end{equation}\n",
    "in Cyclindrical Coordinates\n",
    "\\begin{equation}\n",
    "\\frac {\\partial^2 u}{\\partial \\rho^2} + \\frac{1}{\\rho} \\frac {\\partial u}{\\partial \\rho} + \n",
    "\\frac{1}{\\rho^2} \\frac {\\partial^2 u}{\\partial \\phi^2} = \\frac {\\partial u}{\\partial t}\n",
    "\\end{equation}\n",
    "\n",
    "The radius of the disk will be a.\n",
    "\n",
    "The boundary conditions are\n",
    "u(a, $\\phi$, t) = constant\n",
    "u($\\rho$, 0, t) = u($\\rho$, 0 + 2 $\\pi$, t)\n",
    "\n",
    "Leveraging the Separation of Variables (SOR) approach, we will assume that there is a solution that is the product of 3 functions, each independent in the 3 variables $\\rho, \\phi$ and t.  This means\n",
    "$u(\\rho, \\phi, t) = R(\\rho) \\Phi(\\phi) T(t) $\n",
    "\n",
    "\n",
    "Substituting the solution into the PDE \n",
    "\\begin{equation}\n",
    "\\frac {d^2 R(\\rho)}{d \\rho^2} \\Phi(\\phi) T(t) + \\frac{1}{\\rho} \\frac {d R(\\rho)}{d \\rho} \\Phi(\\phi) T(t) + \n",
    "\\frac{1}{\\rho^2} \\frac {d^2 \\Phi}{ \\phi^2} R(\\rho) T(t) = \\frac {d T(t)}{d t} R(\\rho) \\Phi(\\phi) \n",
    "\\end{equation}\n",
    "\n",
    "Divide both sides by $R(\\rho) \\Phi(\\phi) T(t)$\n",
    "\\begin{equation}\n",
    "\\frac {\\frac {d^2 R(\\rho)}{d \\rho^2} \\Phi(\\phi) T(t) + \\frac{1}{\\rho} \\frac {d R(\\rho)}{d \\rho} \\Phi(\\phi) T(t) + \n",
    "\\frac{1}{\\rho^2} \\frac {d^2 \\Phi}{ \\phi^2} R(\\rho) T(t)} {R(\\rho) \\Phi(\\phi) T(t)} = \\frac{\\frac {d T(t)}{d t} R(\\rho) \\Phi(\\phi)} {{R(\\rho) \\Phi(\\phi) T(t)}} \n",
    "\\end{equation}\n",
    "\\begin{equation}\n",
    "\\frac {\\frac {d^2 R(\\rho)}{d \\rho^2} + \\frac{1}{\\rho} \\frac{d R(\\rho)}{d \\rho}} {R(\\rho) }  + \n",
    "\\frac {\\frac{1}{\\rho^2} \\frac {d^2 \\Phi}{ \\phi^2} } {\\Phi(\\phi)} = \\frac{\\frac {d T(t)}{d t}}{T(t)} \n",
    "\\end{equation}\n",
    "\n",
    "We see that the right-hand side of the equation is comprised of t only.  So, it stands that the left-hand side will change at the same rate as the right-hand side, so we will set it to equal to $\\lambda $\n",
    "\n",
    "\\begin{equation}\n",
    "\\frac {\\frac {d^2 R(\\rho)}{d \\rho^2} + \\frac{1}{\\rho} \\frac{d R(\\rho)}{d \\rho}} {R(\\rho) }  + \n",
    "\\frac {\\frac{1}{\\rho^2} \\frac {d^2 \\Phi}{ \\phi^2} } {\\Phi(\\phi)} = \\frac{\\frac {d T(t)}{d t}}{T(t)} = - \\lambda\n",
    "\\end{equation}\n",
    "\n",
    "Solving the ordinary differential equation in time\n",
    "\\begin{equation}\n",
    "\\frac{\\frac {d T(t)}{d t}}{T(t)} = - \\lambda\n",
    "\\end{equation}\n",
    "\\begin{equation}\n",
    "\\frac {d T(t)}{d t} + \\lambda T(t) = 0\n",
    "\\end{equation}\n",
    "\n",
    "The solution is going to be \n",
    "\\begin{equation}\n",
    "T(t) = C_{0} e ^ {- \\lambda t}\n",
    "\\end{equation}\n",
    "\n",
    "Before we can create 2 separate ordinary differential equations for R($\\rho$) and $\\Phi(\\phi)$ we need to do some work to isolate them.\n",
    "\\begin{equation}\n",
    "\\frac {\\frac {d^2 R(\\rho)}{d \\rho^2} + \\frac{1}{\\rho} \\frac{d R(\\rho)}{d \\rho}} {R(\\rho) }  + \n",
    "\\frac {\\frac{1}{\\rho^2} \\frac {d^2 \\Phi}{d \\phi^2} } {\\Phi(\\phi)} = - \\lambda\n",
    "\\end{equation}\n",
    "By rearranging terms\n",
    "\\begin{equation}\n",
    "\\frac {\\frac {d^2 R(\\rho)}{d \\rho^2} + \\frac{1}{\\rho} \\frac{d R(\\rho)}{d \\rho}}{R(\\rho)}  + \n",
    "\\lambda = - \\frac{\\frac{1}{\\rho^2} \\frac{d^2 \\Phi}{d \\phi^2}}{\\Phi(\\phi)} \n",
    "\\end{equation}\n",
    "and multiplying both sides by $\\rho^2$\n",
    "\\begin{equation}\n",
    "\\frac {\\rho^2 \\frac {d^2 R(\\rho)}{d \\rho^2} + {\\rho} \\frac{d R(\\rho)}{d \\rho}} {R(\\rho)}  + \n",
    "\\rho^2 \\lambda = - \\frac{\\frac {d^2 \\Phi}{d \\phi^2}}{\\Phi(\\phi)}\n",
    "\\end{equation}\n",
    "\n",
    "It follows that this implies, in order for the left and right hand sides to be equal, they must equal a constant that will be assigned to $\\mu$.\n",
    "\\begin{equation}\n",
    "\\rho^2 \\frac {1}{R(\\rho)} \\frac {d^2 R(\\rho)}{d \\rho^2} + \\rho \\frac{1}{R(\\rho)} \\frac{d R(\\rho)}{d \\rho}   + \n",
    "\\rho^2 \\lambda = - \\frac{1}{\\Phi(\\phi)} \\frac{d^2 \\Phi}{d \\phi^2}  = \\mu\n",
    "\\end{equation}\n",
    "\n",
    "Now we can start by solving the the equation in $\\Phi(\\phi)$ first.\n",
    "\\begin{equation}\n",
    "\\frac{1}{\\Phi(\\phi)} \\frac{d^2 \\Phi}{d \\phi^2}  = -\\mu\n",
    "\\end{equation}\n",
    "or \n",
    "\\begin{equation}\n",
    "\\frac{d^2 \\Phi}{d \\phi^2} + \\mu \\Phi(\\phi) = 0\n",
    "\\end{equation}\n",
    "\n",
    "We have to analyze the following conditions:  $\\mu < 0, \\mu = 0, \\mu > 0$ given the periodic boundary conditions:\n",
    "\\begin{equation}\n",
    "\\begin{split}\n",
    "\\Phi(- \\pi) &= \\Phi( \\pi) \\\\\n",
    "\\frac {d\\Phi(- \\pi)}{d \\phi} & = \\frac {d \\Phi( \\pi)}{d \\phi}\n",
    "\\end{split}\n",
    "\\end{equation}\n",
    "\n",
    "For $\\mu = 0 $ :\n",
    "\\begin{equation}\n",
    "\\begin{split}\n",
    "\\frac{d^2 \\Phi}{d \\phi^2} + \\mu \\Phi(\\phi) = 0 \\\\\n",
    "\\text{becomes:  } \\Phi(\\phi) = C_0 + C_1 \\phi \\\\\n",
    "\\text{applying the boundary conditions:  } \\\\ \n",
    "\\Phi(\\pi) = \\Phi(- \\pi) \\\\\n",
    "C_0 + C_1 \\pi = C_0 - C_1 \\pi \\\\\n",
    "\\text{implies } \\\\\n",
    "2  C_1 \\pi = 0 \\\\\n",
    "\\text{or } \\\\\n",
    "C_1 = 0 \\\\ \n",
    "\\text{so there is one solution for $\\mu$ = 0: }\n",
    "\\Phi(\\phi) = C_0 \n",
    "\\end{split}\n",
    "\\end{equation}-\n",
    "\n",
    "For $\\mu < 0 $ :\n",
    "\\begin{equation}\n",
    "\\begin{split}\n",
    "\\frac{d^2 \\Phi}{d \\phi^2} + \\mu \\Phi(\\phi) &= 0 \\\\\n",
    "\\Phi(\\phi) &= C_2 e^{\\sqrt{\\mu}\\phi} + C_3 e^{\\sqrt{\\mu}\\phi} \\\\\n",
    "\\text{since $\\mu$ < 0, the $\\sqrt{\\mu}$ is complex:  } \\\\\n",
    "\\Phi(\\phi) &= C_2 (e^{-i \\sqrt{\\mu}\\phi} + e^{i \\sqrt{\\mu}\\phi}) + C_3 (e^{i \\sqrt{\\mu}\\phi} + e^{-i \\sqrt{\\mu}\\phi}) \\\\\n",
    " &= (C_2 + C_3)e^{-i \\sqrt{\\mu}\\phi} +(C_2 + C_3) e^{i \\sqrt{\\mu}\\phi} \\\\\n",
    " &= C_4 e^{-i \\sqrt{\\mu}\\phi} + C_5 e^{i \\sqrt{\\mu}\\phi} \\\\\n",
    " &= C_4 (\\cos(\\sqrt{\\mu}\\phi) + i \\sin(\\sqrt{\\mu}\\phi)) + C_5 (\\cos(\\sqrt{\\mu}\\phi) + i \\sin(-\\sqrt{\\mu}\\phi))  \\\\\n",
    " &= (C_4 + C_5) \\cos(\\sqrt{\\mu}\\phi) + (C_4 - C_5) i \\sin(\\sqrt{\\mu}\\phi) \\\\\n",
    " &= C_6 \\cos(\\sqrt{\\mu}\\phi) + C_7 \\sin(\\sqrt{\\mu}\\phi) \\\\\n",
    "\\text{applying the boundary conditions:  } \\\\\n",
    "\\Phi(\\pi) &= \\Phi(- \\pi) \\\\\n",
    "C_6 \\cos(\\sqrt{\\mu}\\pi) + C_7 \\sin(\\sqrt{\\mu}\\pi) &= C_6 \\cos(-\\sqrt{\\mu}\\pi) + C_7 \\sin(-\\sqrt{\\mu}\\pi)  \\\\\n",
    "\\text{applying the identities $\\sin(-x)$ = -$\\sin(x)$ and $\\cos(-x)$ = $\\cos(x)$ :  } \\\\\n",
    "C_6 \\cos(\\sqrt{\\mu}\\pi) + C_7 \\sin(\\sqrt{\\mu}\\pi) &= C_6 \\cos(\\sqrt{\\mu}\\pi) - C_7 \\sin(\\sqrt{\\mu}\\pi)  \\\\\n",
    "\\text{combining terms:  } \\\\\n",
    "2 C_7 \\sin(\\sqrt{\\mu}\\pi) &= 0  \\\\\n",
    "C_7 \\sin(\\sqrt{\\mu}\\pi) &= 0 \n",
    "\\end{split}\n",
    "\\end{equation}\n",
    "\n",
    "The next step is to determine the non-trivial solutions;  that is find the eigenvalues so that the sine term evaluates to 0. \n",
    "This will happen when $\\sqrt{\\mu}\\pi$ is a multiple of $\\pi$ or \n",
    "\n",
    "\\begin{equation}\n",
    "\\begin{split}\n",
    "\\sqrt{\\mu}\\pi = m \\pi  \\text{     where m = 1, 2, 3, ... } \\\\\n",
    "\\text{To simplify, we will set $\\sqrt{\\mu} = m$ or $\\mu = m^2$ } \\\\\n",
    "\\therefore \\\\\n",
    "\\Phi(\\phi) &= C \\sin(m \\phi)\n",
    "\\end{split}\n",
    "\\end{equation}\n",
    "\n",
    "For $\\mu > 0 $ :\n",
    "\\begin{equation}\n",
    "\\begin{split}\n",
    "\\frac{d^2 \\Phi}{d \\phi^2} + \\mu \\Phi(\\phi) &= 0 \\\\\n",
    "\\Phi(\\phi) &= C_2 e^{\\sqrt{\\mu}\\phi} + C_3 e^{-\\sqrt{\\mu}\\phi} \\\\\n",
    "\\text{since $\\mu$ > 0, the $\\sqrt{\\mu}$ is real:  } \\\\\n",
    "\\Phi(\\phi) &= C_2 (e^{-\\sqrt{\\mu}\\phi} + e^{\\sqrt{\\mu}\\phi}) + C_3 (e^{\\sqrt{\\mu}\\phi} + e^{-\\sqrt{\\mu}\\phi}) \\\\\n",
    "\\text{since $\\cosh(x)$ = $\\frac{e^x + e^{-x}}{2}$} \\\\\n",
    "&= 2 C_2 \\cosh(\\sqrt{\\mu}\\phi) + 2 C_3 \\cosh(\\sqrt{\\mu}\\phi) \\\\ \n",
    "&= C_4 \\cosh(\\sqrt{\\mu}\\phi) \\\\\n",
    "\\text{or }\n",
    "&= C_4 \\cosh(m\\phi) \\\\\n",
    "\\text{applying the boundary condition:  } \\\\\n",
    "\\Phi(\\pi) &= \\Phi(-\\pi) \\\\\n",
    "C_4 \\cosh(m\\pi) &= C_4 \\cosh(-m\\pi) \\\\\n",
    "\\text{since $\\cosh(-x) = \\cosh(x)$, we do not get a useful answer - only an identity} \\\\\n",
    "\\text{However, when m $\\rightarrow \\infty$, $\\cosh(x) \\rightarrow \\infty$ }\\\\\n",
    "&= C_4 \\cosh(m\\phi) \\rightarrow \\infty \\\\\n",
    "\\text{and this requires $C_4$ = 0 because the function needs to be bounded.}\n",
    "\\end{split}\n",
    "\\end{equation}\n",
    "\n",
    "Therefore, after considering the three conditions  $\\mu < 0, \\mu = 0, \\mu > 0$, and using the superposition:\n",
    "\\begin{equation}\n",
    "\\begin{split}\n",
    "\\Phi(\\phi) &= C_0 + C \\sin(m \\phi) \\text{    where m = 1, 2, 3, ...} \\\\\n",
    "\\text{because each value of m is a solution, we need to sum all of these solutions } \\\\\n",
    "\\Phi(\\phi) &= C_0 + \\sum_{m=1}^{\\infty}{C_m \\sin(m \\phi)} \n",
    "\\end{split}\n",
    "\\end{equation}\n",
    "\n",
    "We have solved the components for time T(t) and $\\Phi(\\phi)$, and the last step will be to solve the radial equation $R(rho)$.\n",
    "\\begin{equation}\n",
    "\\begin{split}\n",
    "\\rho^2 \\frac {1}{R(\\rho)} \\frac {d^2 R(\\rho)}{d \\rho^2} + \\rho \\frac{1}{R(\\rho)} \\frac{d R(\\rho)}{d \\rho}   + \n",
    "\\rho^2 \\lambda &= \\mu \\\\\n",
    "\\rho^2 \\frac {1}{R(\\rho)} \\frac {d^2 R(\\rho)}{d \\rho^2} + \\rho \\frac{1}{R(\\rho)} \\frac{d R(\\rho)}{d \\rho}   + \n",
    "\\rho^2 \\lambda - \\mu &= 0 \\\\\n",
    "\\text{Multiply through by $R(\\rho)$,} \\\\\n",
    "\\rho^2  \\frac {d^2 R(\\rho)}{d \\rho^2} + \\rho \\frac{d R(\\rho)}{d \\rho} + \\rho^2 \\lambda R(\\rho) - \\mu R(\\rho) &= 0 \\\\\n",
    "\\rho^2  \\frac {d^2 R(\\rho)}{d \\rho^2} + \\rho \\frac{d R(\\rho)}{d \\rho} + (\\rho^2 \\lambda - \\mu)R(\\rho) &= 0 \\\\\n",
    "\\text{since $\\mu$ = $m^2$} \\\\\n",
    "\\rho^2  \\frac {d^2 R(\\rho)}{d \\rho^2} + \\rho \\frac{d R(\\rho)}{d \\rho} + (\\rho^2 \\lambda - m^2)R(\\rho) &= 0\n",
    "\\end{split}\n",
    "\\end{equation}\n",
    "The resulting differential equation is a Bessel function.  The derivation can be found here.\n",
    "\n",
    "The complete solution is therefore:\n",
    "\\begin{equation}\n",
    "\\begin{split}\n",
    "u(\\rho, \\phi, t) &= R(\\rho) \\Phi(\\phi) T(t) \\\\\n",
    "R(\\rho) &= J_0(\\rho j_{n}) \\>\\>\\>\\>\\>\\>\\>\\> n = 1, 2, 3, \\cdots \\\\\n",
    "&= c J_{m}(\\rho j_{m,n})  \\>\\> m, n = 1, 2, 3, \\cdots \\\\\n",
    "\\Phi(\\phi) &= \\sum_{m=1}^{\\infty} C_0 + {C_m \\sin(m \\phi)} \\\\\n",
    "T(t) &= C_{0} e ^ {- \\lambda t} = C_{0} e ^ {- j_{m,n}^2 t}  \\\\\n",
    "u(\\rho, \\phi, t) &= \\sum_{m=1}^{\\infty} \\sum_{n=1}^{\\infty} c J_{m}(\\rho j_{m,n}) \\cdot \\left(C_0 + {C_m \\sin(m \\phi)} \\right) \\cdot  C_{0} e ^ {- \\lambda t} \\\\\n",
    "&= \\sum_{m=1}^{\\infty} \\sum_{n=1}^{\\infty} J_{m}(\\rho j_{m,n}) \\cdot \\left(C_0 + {C_m \\sin(m \\phi)} \\right) \\cdot  C_{0} e ^ {- j_{m,n}^2 t} \\\\\n",
    "&= \\sum_{m=1}^{\\infty} \\sum_{n=1}^{\\infty} C {J_{m}(\\rho j_{m,n}) \\cdot \\left(C_0 + {\\sin(m \\phi)} \\right) \\cdot e ^ {- j_{m,n}^2 t} }\n",
    "\\end{split}\n",
    "\\end{equation}\n"
   ]
  },
  {
   "cell_type": "code",
   "execution_count": null,
   "id": "533b12de",
   "metadata": {},
   "outputs": [],
   "source": []
  },
  {
   "cell_type": "code",
   "execution_count": null,
   "id": "e83d7d6f",
   "metadata": {},
   "outputs": [],
   "source": []
  }
 ],
 "metadata": {
  "kernelspec": {
   "display_name": "Python 3",
   "language": "python",
   "name": "python3"
  },
  "language_info": {
   "codemirror_mode": {
    "name": "ipython",
    "version": 3
   },
   "file_extension": ".py",
   "mimetype": "text/x-python",
   "name": "python",
   "nbconvert_exporter": "python",
   "pygments_lexer": "ipython3",
   "version": "3.9.1"
  },
  "toc": {
   "base_numbering": 1,
   "nav_menu": {},
   "number_sections": true,
   "sideBar": true,
   "skip_h1_title": false,
   "title_cell": "Table of Contents",
   "title_sidebar": "Contents",
   "toc_cell": false,
   "toc_position": {},
   "toc_section_display": true,
   "toc_window_display": false
  },
  "varInspector": {
   "cols": {
    "lenName": 16,
    "lenType": 16,
    "lenVar": 40
   },
   "kernels_config": {
    "python": {
     "delete_cmd_postfix": "",
     "delete_cmd_prefix": "del ",
     "library": "var_list.py",
     "varRefreshCmd": "print(var_dic_list())"
    },
    "r": {
     "delete_cmd_postfix": ") ",
     "delete_cmd_prefix": "rm(",
     "library": "var_list.r",
     "varRefreshCmd": "cat(var_dic_list()) "
    }
   },
   "types_to_exclude": [
    "module",
    "function",
    "builtin_function_or_method",
    "instance",
    "_Feature"
   ],
   "window_display": false
  }
 },
 "nbformat": 4,
 "nbformat_minor": 5
}
